---
author: "Daniel Wysocki and Kenny Roffo"
title: "Quantum Harmonic Oscillator"
date: "February 26, 2015"
output:
  beamer_presentation:
    theme: "Madrid"
    colortheme: "dolphin"
    fonttheme: "serif"
    includes:
      in_header: [header.tex]
---

# The Harmonic Oscillator

- the classic example of a harmonic oscillator in classical mechanics is a
  mass $m$ attached to a spring with spring constant $k$
$$F = -kx = m \dod[2]{x}{t}$$
- this is an ODE with solution
$$x(t) = A \sin(\omega t) + B \cos(\omega t),$$
- where $\omega = \sqrt{k / m}$

# The Harmonic Oscillator Potential

- the potential energy is parabolic, and given by $V(x) = \frac{1}{2} k x^2$,
- practically any potential is approximately parabolic, when $x$ is close to
  some local minimum, $x_0$
- this can be shown by the taylor series centered around $x_0$


# The Harmonic Oscillator Potential

$$V(x) = V(x_0) + V'(x_0)(x-x_0) + \frac{1}{2} V''(x_0)(x-x_0)^2 + \ldots$$

- ignore the constant $V(x_0)$, as that has no effect on the force
- $V'(x_0) = 0$, because it is a local minimum
- ignore the higher order terms, leaving
$$V(x) \cong \frac{1}{2} V''(x_0) (x-x_0)^2$$


# Ladder Operators

- the time independent Schrödinger equation is given by
$$-\frac{\hbar^2}{2 m} \dod[2]{\psi}{x} + V(x) \psi = E \psi$$
- using $\hat{p}^2 = -\hbar^2 \od[2]{}{x}$,
  and $V(x) = \frac{1}{2} m \omega^2 x^2$, we can rewrite the wave equation as
$$\frac{1}{2 m} \left[ \hat{p}^2 + (m \omega x)^2 \right] \psi = E \psi$$
- so the Hamiltonian is
$$\hat{H} = \frac{1}{2 m} \left[ \hat{p}^2 + (m \omega x)^2 \right]$$



# Ladder Operators

- if $\hat{p}$ were a scalar, and not an operator, then we could rewrite the
  Hamiltonian as
$$\hat{H} = \frac{1}{2 m}
  (\imath \hat{p} + m \omega x) (-\imath \hat{p} + m \omega x)$$
- this is obviously false, but it is still worth inspecting this quantity on
  the left
- to make the math simpler later, we multiply by $1/(\hbar\omega)$
$$\frac{1}{2 \hbar m \omega}
  (\imath \hat{p} + m \omega x) (-\imath \hat{p} + m \omega x)$$

$$\left[ \frac{1}{\sqrt{2 \hbar m \omega}}(\imath \hat{p} + m \omega x)  \right]
\left[ \frac{1}{\sqrt{2 \hbar m \omega}}(-\imath \hat{p} + m \omega x) \right]
:= a_- a_+$$


# Ladder Operators

- we have just defined the raising operator ($a_+$) and the lowering operator
  ($a_-$)
$$a_\pm :=
  \frac{1}{\sqrt{2 \hbar m \omega}} [\mp \imath \hat{p} + m \omega x]$$
- remember, if $\hat{p}$ behaved like a number, then
  $a_- a_+ = 1/(\hbar \omega) \hat{H}$
- let us now see what $a_- a_+$ *actually* is


# Product of Ladder Operators

\begin{align*}
a_- a_+ &=
\frac{1}{2 \hbar m \omega}
(\imath \hat{p} + m \omega x)
(-\imath \hat{p} + m \omega x)
\\ &=
\frac{1}{2 \hbar m \omega}
[\hat{p}^2 + (m \omega x)^2 - \imath m \omega (x \hat{p} - \hat{p} x)]
\\ &=
\frac{1}{2 \hbar m \omega}
[\hat{p}^2 + (m \omega x)^2 - \imath m \omega [x, \hat{p}]]
\\ &=
\frac{1}{2 \hbar m \omega}
[\hat{p}^2 + (m \omega x)^2 - \imath m \omega (\imath \hbar)]
\\ &=
\frac{1}{2 \hbar m \omega} [\hat{p}^2 + (m \omega x)^2] + \frac{1}{2}
\\ &=
\frac{1}{\hbar \omega} \hat{H} + \frac{1}{2}
\end{align*}


# Hamiltonian in Terms of Ladder Operators

- we have just shown
$$a_- a_+ = \frac{1}{\hbar \omega} \hat{H} + \frac{1}{2}$$
- solving for $\hat{H}$ gives
$$\hat{H} = \hbar \omega \left( a_- a_+ - \frac{1}{2} \right)$$
- working out the derivation on the previous slide again, with the order of
  operators reversed gives
$$\hat{H} = \hbar \omega \left( a_+ a_- + \frac{1}{2} \right)$$


# Raising Operator

- $\psi$ satisfies the Schrödinger equation with energy $E$
$$\hat{H} \psi = E \psi$$
- now we will show that $a_+ \psi$ satisfies the Schrödinger equation with
  energy $E + \hbar\omega$

# Raising Operator

\begin{align*}
\hat{H} (a_+ \psi) &=
\hbar \omega \left( a_+ a_- + \frac{1}{2} \right) (a_+ \psi) =
\hbar \omega \left( a_+ a_- a_+ + \frac{1}{2} a_+ \right) \psi
\\ &=
\hbar \omega a_+ \left( a_- a_+ + \frac{1}{2} \right) \psi =
a_+ \left[ \hbar \omega \left( a_+ a_- + \frac{1}{2} + 1 \right) \psi \right]
\\ &=
a_+ (\hat{H} + \hbar \omega) \psi =
a_+ (E + \hbar \omega) \psi =
(E + \hbar \omega) (a_+ \psi).
\end{align*}


# Lowering Operator

\begin{align*}
\hat{H} (a_- \psi) &=
\hbar \omega \left( a_- a_+ - \frac{1}{2} \right) (a_- \psi) =
\hbar \omega \left( a_- a_+ a_- - \frac{1}{2} a_- \right) \psi
\\ &=
\hbar \omega a_- \left( a_+ a_- - \frac{1}{2} \right) \psi =
a_- \left[ \hbar \omega \left( a_- a_+ - \frac{1}{2} - 1 \right) \psi \right]
\\ &=
a_- (\hat{H} - \hbar \omega) \psi =
a_- (E - \hbar \omega) \psi =
(E - \hbar \omega) (a_- \psi).
\end{align*}


# The Lowest Rung

- if we apply the lowering operator repeatedly, eventually we will reach a
  negative energy
- however, there occurs a point where $a_- \psi_0 = 0$
    - this is non-normalizable, and therefore an invalid solution
- this helps us determine $\psi_0(x)$
$$\frac{1}{\sqrt{2 \hbar m \omega}}
  \left( \hbar \dod{}{x} + m \omega x \right) \psi_0 =
  0$$
$$\psi_0(x) =
  \sqrt[4]{\frac{m \omega}{\pi \hbar}} \exp(-\frac{m \omega}{2 \hbar} x^2)$$

# Solution to All Stationary States

- recursive solution
\begin{align*}
\psi_0(x) &=
\sqrt[4]{\frac{m \omega}{\pi \hbar}} \exp(-\frac{m \omega}{2 \hbar} x^2)
\\
\psi_n(x) &=
A_n (a_+)^n \psi_0(x), \quad
\text{ with }
E_n = \left( n + \frac{1}{2} \right) \hbar \omega
\end{align*}
- we can solve for the normalization constant $A_n$ individually for each
  solution, but it turns out that
$$A_n = \frac{1}{\sqrt{n!}}$$



# Thank you!
